\input{src/137.tex}

\D 1 Так как $\pb{(e^x)}k = e^x,\s \pb{(e^x)}k|_{x = 0} = 1$.

\D2 Из формулы \FF{\pb{\sin x}m = \sin(x + \frac \pi2) } при $k \in \Z_+$ находим \FF{\pb{\sin x}{2k}|_{x = 0} = 0,\quad \pb{(\sin(x))}{2k + 1}|_{x = 0} = (-1)^k. }

\D4 Поскольку при всех $k \in \N$ \FF{\pb{\ln(1 + x)}k = \frac{(-1)^{k - 1}(k - 1)!}{(1 + x)^k},\quad \pb{(\ln(1 + x))}k|_{x = 0} = (-1)^{k - 1}(k - 1)! ,} а $\ln 1 = 0$, получаем формулу.

\D5 Пусть $\alpha \in \R$. Положим \FF{C^k_n = \frac{\alpha(\alpha - 1)\cdot(\alpha - k + 1)}{k!},\quad k \in Z_+ .} Тогда поучаем формулу.